Formalize the behavior of TMs before they write their first non-zero symbol

verify/Enumerate.v
@@ -1,7 +1,10 @@
 (** * Enumerate: TNF enumeration *)
 
 From Coq Require Import List. Import ListNotations.
+From Coq Require Import Lists.Streams.
+From Coq Require Import Lia.
 From BusyCoq Require Export Permute.
+From BusyCoq Require Import Pigeonhole.
 Set Default Goal Selector "!".
 
 Module Enumerate (Ctx : Ctx).
@@ -12,44 +15,59 @@ Module Enumerate (Ctx : Ctx).
     their first 1 (or a non-zero symbol in the case of non-binary Turing
     machines). *)
 
+Inductive ReachedNZ (tm : TM) : Q -> Prop :=
+  | reached_halt q :
+    tm (q, s0) = None ->
+    ReachedNZ tm q
+  | reached_nz q s d q' :
+    tm (q, s0) = Some (s, d, q') ->
+    s <> s0 ->
+    ReachedNZ tm q.
+
 (** [tm] visits the sequence of states [q :: qs] before writing its first
     non-zero symbol. *)
 Inductive zvisits (tm : TM) : Q -> list Q -> Prop :=
-  | zvisits_halt q :
-    tm (q, s0) = None ->
-    zvisits tm q []
-  | zvisits_nz q s d q' :
-    tm (q, s0) = Some (s, d, q') ->
-    s <> s0 ->
+  | zvisits_done q :
+    ReachedNZ tm q ->
     zvisits tm q []
   | zvisits_step q d q' qs :
     tm (q, s0) = Some (s0, d, q') ->
     zvisits tm q' qs ->
     zvisits tm q (q' :: qs).
 
-(** This sequence is unique. *)
+Local Hint Constructors ReachedNZ zvisits : core.
 
-Lemma zvisits_unique : forall tm qs qs' q,
+(** This sequence is unique for each [q]. *)
+Lemma zvisits_unique : forall {tm qs qs' q},
   zvisits tm q qs ->
   zvisits tm q qs' ->
   qs = qs'.
 Proof.
   induction qs as [| a qs IH]; introv H1 H2;
-    inverts H1; inverts H2; try congruence.
+    inverts H1; inverts H2;
+    try lazymatch goal with
+    | H: ReachedNZ _ _ |- _ => inverts H
+    end;
+    try congruence.
   assert (a = q'). { congruence. }
   subst. f_equal. eauto.
 Qed.
 
-(** Therefore, [q] cannot occur in [qs]. *)
-Lemma zvisits_In_skip : forall tm qs q q',
+(** Therefore, [q] cannot occur in [qs] – otherwise a suffix would
+    violate uniqueness. *)
+Lemma zvisits_In_skipn : forall {tm qs q q'},
   zvisits tm q qs ->
   In q' qs ->
-  exists qs', zvisits tm q' qs' /\ qs <> qs'.
+  exists n, zvisits tm q' (skipn (S n) qs).
 Proof.
   induction qs as [| a qs IH].
   - contradiction.
   - introv Hvisits Hin. inverts Hvisits as Etm Hvisits.
-    destruct Hin as [E | Hin]; subst; eauto.
+    destruct Hin as [E | Hin].
+    + subst a. exists 0. auto.
+    + specialize (IH _ _ Hvisits Hin).
+      destruct IH as [n IH].
+      exists (S n). auto.
 Qed.
 
 Lemma zvisits_In : forall tm qs q,
@@ -57,9 +75,96 @@ Lemma zvisits_In : forall tm qs q,
   ~ In q qs.
 Proof.
   introv H1 Hin.
-  apply 
-  induction qs as [| a qs IH].
-  - contradiction.
-  - inverts H1 as Etm H1.
-    * subst a.
-  assert (H2: zvisits tm 
+  destruct (zvisits_In_skipn H1 Hin) as [n H2].
+  pose proof (zvisits_unique H1 H2) as E.
+  assert (E': length qs = length (skipn (S n) qs)).
+  { f_equal. exact E. }
+  rewrite skipn_length in E'.
+  assert (Hqs : length qs = 0) by lia.
+  apply length_zero_iff_nil in Hqs. subst qs.
+  exact Hin.
+Qed.
+
+(** Hence, elements in [qs] do not repeat. *)
+Lemma zvisits_not_repeats : forall tm qs q,
+  repeats qs ->
+  ~ zvisits tm q qs.
+Proof.
+  introv H. generalize dependent q.
+  induction H; introv Hvisits.
+  - (* repeats_head *)
+    inverts Hvisits as E Hvisits.
+    apply zvisits_In in Hvisits. contradiction.
+  - (* repeats_cons *)
+    inverts Hvisits as E Hvisits.
+    apply IHrepeats in Hvisits. contradiction.
+Qed.
+
+(** We can say more: the elements in [q :: qs] do not repeat. *)
+Lemma zvisits_not_repeats' : forall tm qs q,
+  zvisits tm q qs ->
+  ~ repeats (q :: qs).
+Proof.
+  introv Hvisits Hrepeats.
+  inverts Hrepeats as H.
+  - (* repeats_head *)
+    apply zvisits_In in Hvisits. contradiction.
+  - (* repeats_cons *)
+    eapply zvisits_not_repeats in H. eauto.
+Qed.
+
+Proposition zvisits_bound : forall tm q qs,
+  zvisits tm q qs ->
+  length qs < length all_qs.
+Proof.
+  introv Hvisits.
+  enough (~ length all_qs <= length qs) by lia.
+  introv Hpigeon.
+  assert (Hrepeats : repeats (q :: qs)).
+  { apply pigeonhole_principle with all_qs.
+    - apply <- Forall_forall. auto.
+    - simpl. lia. }
+  apply zvisits_not_repeats' in Hvisits.
+  contradiction.
+Qed.
+
+(** Any halting machine has a [zvisits] sequence. *)
+Proposition halts_zvisits : forall tm q,
+  halts tm (q;; tape0) ->
+  exists qs, zvisits tm q qs.
+Proof.
+  introv Hhalts.
+  destruct Hhalts as [k [ch [Hsteps Hhalted]]].
+  remember (q;; tape0) as c.
+  generalize dependent q.
+  induction Hsteps as [| n c c' ch Hstep Hrest IH]; introv E; subst c.
+  - eauto.
+  - inverts Hstep as Etm;
+    destruct (eqb_sym s' s0) as [E | E]; subst; eauto;
+    fold tape0 in *; autorewrite with tape in *;
+    specialize (IH Hhalted q' eq_refl);
+    destruct IH as [qs IH]; eauto.
+Qed.
+
+Lemma zero_step : forall tm q d q',
+  tm (q, s0) = Some (s0, d, q') ->
+  q;; tape0 -[ tm ]-> q';; tape0.
+Proof with constructor; assumption.
+  introv E.
+  destruct d.
+  - rewrite <- move_left_tape0 at 2...
+  - rewrite <- move_right_tape0 at 2...
+Qed.
+
+Local Hint Resolve zero_step : core.
+
+(** [zvisits] corresponds to what the Turing machine actually does *)
+Proposition zvisits_steps : forall tm q qs,
+  zvisits tm q qs ->
+  exists q', q;; tape0 -[ tm ]->> length qs / q';; tape0 /\ ReachedNZ tm q'.
+Proof.
+  introv H. induction H.
+  - eauto.
+  - destruct IHzvisits as [q'' [IH1 IH2]].
+    simpl. eauto.
+Qed.
